example/out/ProcDecExec.v
@@ -2,85 +2,63 @@ Require Import Bool String List Arith.
 Require Import Omega.
 Require Import Kami.All.
 Require Import Bsvtokami.
-Require Import Decoder.
 
 Require Import FunctionalExtensionality.
 
 Set Implicit Arguments.
 
 
+Require Import Decoder.
 Require Import FIFO.
 Require Import RegFile.
 Require Import ProcMemSpec.
-Require Import PipelinedProc.
-Require Import Vector.
+(* * interface NoMethods *)
+Record NoMethods := {
+    NoMethods'mod: ModWf;
+}.
+
+Hint Unfold NoMethods'mod : ModuleDefs.
+
 Module module'mkDecExec.
     Section Section'mkDecExec.
     Variable instancePrefix: string.
-    Variable dec: Decoder.Decoder.
+    Variable pgm: string.
+    Variable dec: string.
     Variable exec: Decoder.Executer.
+    Variable e2wfifo: string.
         (* method bindings *)
-    Let pc : string := instancePrefix--"pc".
-    (* Let sbFlags : string := instancePrefix--"sbFlags". *)
-    Let rf: string := instancePrefix--"rf".
-    Let mem: string := instancePrefix--"mem".
-    Let pgm: string := "pgm".
-    Let toHost: string := instancePrefix--"th".
-    Let e2wFifo_idx: string := instancePrefix--"e2wFifo_idx".
-    Let e2wFifo_val: string := instancePrefix--"e2wFifo_val".
-    Let e2wFifo_valid: string := instancePrefix--"e2wFifo_valid".
     (* instance methods *)
-    Let mem'doMem : string := mem--"doMem".
-    Let toHost'toHost : string := toHost--"toHost".
     Local Open Scope kami_expr.
 
-    Definition mkDecExecModule: Mod :=
-         (BKMODULE {
-    Register e2wFifo_idx : Bit RegFileSz <- Default
-    with Register e2wFifo_val : Bit DataSz <- Default
-    with Register e2wFifo_valid : Bool <- (false)%kami_expr
-    with Register pc : Bit PgmSz <- natToWord PgmSz 0
-    with Register pgm : Array NumInstrs (Bit InstrSz) <- Default
-    with Register rf : Array NumRegs (Bit DataSz) <- Default
-    (* with Register sbFlags : Array NumRegs Bool <- Default *)
+    Definition mkDecExecModule: ModWf :=
+         (MOD_WF {
+        Register (instancePrefix--"pc") : Bit PgmSz <- Default
+    with Register (instancePrefix--"rf") : Array NumRegs (Bit DataSz) <- Default
     with Rule instancePrefix--"decexecArith" :=
     (
-        Read e2wFifo_valid_v : Bool <- e2wFifo_valid ;
-        Read pc_v : Bit PgmSz <- pc ;
-        (* Read sbFlags_v : Array NumRegs Bool <- sbFlags ; *)
-       Read instrs : Array NumInstrs (Bit InstrSz) <- pgm ;
-       LET inst : Bit InstrSz <- #instrs @[  #pc_v ] ;
-       LET isOpArith : Bool <- (getOp dec _ inst) == $$opArith ;
-       LET src1 : Bit RegFileSz <-  getSrc1 dec _ inst ;
-       LET src2 : Bit RegFileSz <-  getSrc2 dec _ inst ;
+        Read pc_v : Bit PgmSz <- (instancePrefix--"pc") ;
+        Read rf_v : Array NumRegs (Bit DataSz) <- (instancePrefix--"rf") ;
+       (* call expr ProcDecExec.bsv:18 *) BKCall call19 : Bit InstrSz <-  (* translateCall *) (pgm--"sub") ((#pc_v) : Bit PgmSz)  ;
+       (* call expr ProcDecExec.bsv:18 *) BKCall call18 : Bit 2 <-  (* translateCall *) (dec--"getOp") ((#call19) : Bit InstrSz)  ;
 
-        Assert(#isOpArith 
-	(* && !(#sbFlags_v @[ #src1 ]) *)
-	(* && (!(#sbFlags_v @[ #src2 ])) *)
-	 && (!#e2wFifo_valid_v)) ;
-       LET dst : Bit RegFileSz (* varbinding *) <-  getDst dec _ inst ;
-       LET arithOp : OpArithK (* varbinding *) <- getArithOp dec _ inst ;
-       Read regsval : Array NumRegs (Bit DataSz) <- rf ;
-       LET val1 : Bit DataSz (* varbinding *) <-  #regsval @[ #src1 ] ;
-       LET val2 : Bit DataSz (* varbinding *) <-  #regsval @[ #src2 ] ;
-       LET execVal : Bit DataSz <- (execArith exec _ arithOp val1 val2) ;
-       (* LET flags : Array NumRegs Bool (* non-call varbinding *) <- #sbFlags_v ;
-               LET flags : Array NumRegs Bool <- #flags @[#dst <- $$true] ;
-               Write sbFlags : Array NumRegs Bool <- #flags ; *)
-               (* LET e2w : E2W (* non-call varbinding *) <- STRUCT { "idx" ::= (#dst) ; "val" ::= (#execVal)  }%kami_expr ;
-               Write e2wFifo_reg : E2W <- #e2w ; *)
-               Write e2wFifo_idx : Bit RegFileSz <- #dst ;
-               Write e2wFifo_val : Bit DataSz <- #execVal ;
-               Write e2wFifo_valid : Bool <- ($$true)%kami_expr ;
-               Write pc : Bit PgmSz <- (#pc_v + $$ (* intwidth *) (natToWord PgmSz 1)) ;
-        Retv ) (* rule decexecArith *)
+        Assert(#call18 == ($$ (* isConstT *)opArith)) ;
+       BKCall inst : Bit InstrSz (* varbinding *) <-  (* translateCall *) (pgm--"sub") ((#pc_v) : Bit PgmSz)  ;
+       BKCall src1 : Bit RegFileSz (* varbinding *) <-  (* translateCall *) (dec--"getSrc1") ((#inst) : Bit InstrSz)  ;
+       BKCall src2 : Bit RegFileSz (* varbinding *) <-  (* translateCall *) (dec--"getSrc2") ((#inst) : Bit InstrSz)  ;
+       BKCall dst : Bit RegFileSz (* varbinding *) <-  (* translateCall *) (dec--"getDst") ((#inst) : Bit InstrSz)  ;
+       BKCall retval : Bit 2 <- (dec--"getArithOp") ((#inst) : Bit InstrSz)  ;
+      LET arithOp : Bit 2 <- #retval ;
+      LET val1 : Bit DataSz (* non-call varbinding *) <- (#rf_v @[ #src1 ]) ;
+      LET val2 : Bit DataSz (* non-call varbinding *) <- (#rf_v @[ #src2 ]) ;
+      LET execVal : Bit DataSz <- (execArith exec _ arithOp val1 val2)  ;
+      BKCall enq : Void (* actionBinding *) <- (e2wfifo--"enq") ((#execVal) : Bit DataSz)  ;
+      Write (instancePrefix--"pc") : Bit PgmSz <- (#pc_v + $$ (* intwidth *) (natToWord PgmSz 1))  ;
+      Retv ) (* rule decexecArith *)
     }). (* mkDecExec *)
 
-    Close Scope kami_expr.
-
     Hint Unfold mkDecExecModule : ModuleDefs.
-(* Module mkDecExec type RegFile#(Bit#(PgmSz), Bit#(InstrSz)) -> Decoder -> Executer -> Reg#(E2W) -> Reg#(Bool) -> ProcRegs -> Memory -> ToHost -> Module#(Empty) return type Decoder *)
-    Definition mkDecExec := Build_Empty mkDecExecModule.
+(* Module mkDecExec type RegFile#(Bit#(PgmSz), Bit#(InstrSz)) -> Decoder -> Executer -> Module#(NoMethods) return type Decoder *)
+    Definition mkDecExec := Build_NoMethods mkDecExecModule.
     Hint Unfold mkDecExec : ModuleDefs.
     Hint Unfold mkDecExecModule : ModuleDefs.
 
@@ -95,120 +73,64 @@ Hint Unfold module'mkDecExec.mkDecExecModule : ModuleDefs.
 Module module'mkDecExecSep.
     Section Section'mkDecExecSep.
     Variable instancePrefix: string.
-    Variable dec: Decoder.Decoder.
+    Variable pgm: string.
+    Variable dec: string.
     Variable exec: Decoder.Executer.
-        (* method bindings *)
-    Let rf: string := instancePrefix--"rf".
-    Let mem: string := instancePrefix--"mem".
-    Let pgm: string := "pgm".
-    Let toHost: string := instancePrefix--"th".
-    Let d2eFifo_addr    : string := instancePrefix--"d2eFifo_addr".
-    Let d2eFifo_arithOp : string := instancePrefix--"d2eFifo_arithOp".
-    Let d2eFifo_op      : string := instancePrefix--"d2eFifo_op".
-    Let d2eFifo_pc      : string := instancePrefix--"d2eFifo_pc".
-    Let d2eFifo_dst     : string := instancePrefix--"d2eFifo_dst".
-    Let d2eFifo_src1    : string := instancePrefix--"d2eFifo_src1".
-    Let d2eFifo_src2    : string := instancePrefix--"d2eFifo_src2".
-    Let d2eFifo_valid : string := instancePrefix--"d2eFifo_valid".
-    Let e2wFifo_idx : string := instancePrefix--"e2wFifo_idx".
-    Let e2wFifo_val : string := instancePrefix--"e2wFifo_val".
-    Let e2wFifo_valid : string := instancePrefix--"e2wFifo_valid".
-    Let decoder_pc : string := instancePrefix--"pc".
-    (* Let sbFlags : string := instancePrefix--"sbFlags". *)
-    (* instance methods *)
-    Let mem'doMem : string := mem--"doMem".
-    Let toHost'toHost : string := toHost--"toHost".
+    Variable e2wfifo: string.
     Local Open Scope kami_expr.
 
-    Definition mkDecExecSepModule: Mod :=
-         (BKMODULE {
-
-         Register decoder_pc : Bit PgmSz <-  (* intwidth *) (natToWord PgmSz 0)
-
-    with Register d2eFifo_valid : Bool <- (false)%kami_expr
-    with Register d2eFifo_addr    : Bit AddrSz <- Default
-    with Register d2eFifo_arithOp : OpArithK <- Default
-    with Register d2eFifo_op      : OpK <- Default
-    with Register d2eFifo_pc      : Bit PgmSz <- Default
-    with Register d2eFifo_dst     : Bit RegFileSz <- Default
-    with Register d2eFifo_src1    : Bit RegFileSz <- Default
-    with Register d2eFifo_src2    : Bit RegFileSz <- Default
-
-    with Register e2wFifo_idx : Bit RegFileSz <- Default
-    with Register e2wFifo_val : Bit DataSz <- Default
-    with Register e2wFifo_valid : Bool <- (false)%kami_expr
-    with Register pgm : Array NumInstrs (Bit InstrSz) <- Default
-    with Register rf : Array NumRegs (Bit DataSz) <- Default
-    (* with Register sbFlags : Array NumRegs Bool <- Default *)
-
+    Definition mkDecExecSepModule: ModWf :=
+         (MOD_WF {
+    Register (instancePrefix--"pc") : Bit PgmSz <- Default
+    with Register (instancePrefix--"d2e_valid")   : Bool <- Default
+    with Register (instancePrefix--"d2e_pc")      : Bit PgmSz <- Default
+    with Register (instancePrefix--"d2e_op")      : Bit 2 <- Default
+    with Register (instancePrefix--"d2e_arithOp") : Bit 2 <- Default
+    with Register (instancePrefix--"d2e_src1")    : Bit RegFileSz <- Default
+    with Register (instancePrefix--"d2e_src2")    : Bit RegFileSz <- Default
+    with Register (instancePrefix--"d2e_dst")     : Bit RegFileSz <- Default
+    with Register (instancePrefix--"rf") : Array NumRegs (Bit DataSz) <- Default
     with Rule instancePrefix--"decode" :=
     (
-        Read d2eFifo_valid_v : Bool <- d2eFifo_valid ;
-        Read decoder_pc_v : Bit PgmSz <- decoder_pc ;
-
-        Assert((!#d2eFifo_valid_v)) ;
-       Read instrs : Array NumInstrs (Bit InstrSz) <- pgm ;
-       LET inst : Bit InstrSz <- #instrs @[ #decoder_pc_v ] ;
-       LET op : OpK (* varbinding *) <-  getOp dec _ inst ;
-       LET arithOp : OpArithK (* varbinding *) <-  getArithOp dec _ inst ;
-       LET src1 : Bit RegFileSz (* varbinding *) <-  getSrc1 dec _ inst ;
-       LET src2 : Bit RegFileSz (* varbinding *) <-  getSrc2 dec _ inst ;
-       LET dst : Bit RegFileSz (* varbinding *) <-  getDst dec _ inst ;
-       LET addr : Bit AddrSz (* varbinding *) <- getAddr dec _ inst ;
-               Write d2eFifo_addr    : Bit AddrSz    <- #addr ;
-               Write d2eFifo_arithOp : OpArithK      <- #arithOp ;
-               Write d2eFifo_op      : OpK           <- #op ;
-               Write d2eFifo_pc      : Bit PgmSz     <- #decoder_pc_v ;
-               Write d2eFifo_dst     : Bit RegFileSz <- #dst ;
-               Write d2eFifo_src1    : Bit RegFileSz <- #src1 ;
-               Write d2eFifo_src2    : Bit RegFileSz <- #src2 ;
-               Write d2eFifo_valid : Bool <- ($$true)%kami_expr ;
-               Write decoder_pc : Bit PgmSz <- (#decoder_pc_v + $$ (* intwidth *) (natToWord PgmSz 1)) ;
+        Read pc_v : Bit PgmSz <- (instancePrefix--"pc") ;
+       BKCall inst : Bit InstrSz (* varbinding *) <-  (* translateCall *) (pgm--"sub") ((#pc_v) : Bit PgmSz)  ;
+       BKCall op : Bit 2 (* varbinding *) <-  (* translateCall *) (dec--"getOp") ((#inst) : Bit InstrSz)  ;
+       BKCall arithOp : Bit 2 (* varbinding *) <-  (* translateCall *) (dec--"getArithOp") ((#inst) : Bit InstrSz)  ;
+       BKCall src1 : Bit RegFileSz (* varbinding *) <-  (* translateCall *) (dec--"getSrc1") ((#inst) : Bit InstrSz)  ;
+       BKCall src2 : Bit RegFileSz (* varbinding *) <-  (* translateCall *) (dec--"getSrc2") ((#inst) : Bit InstrSz)  ;
+       BKCall dst  : Bit RegFileSz (* varbinding *) <-  (* translateCall *) (dec--"getDst") ((#inst) : Bit InstrSz)  ;
+       Write (instancePrefix--"d2e_valid") : Bool <- $$true ;
+       Write (instancePrefix--"d2e_pc") : Bit PgmSz <- #pc_v ;
+       Write (instancePrefix--"d2e_arithOp") : Bit 2 <- #arithOp ;
+       Write (instancePrefix--"d2e_op") : Bit 2 <- #op ;
+       Write (instancePrefix--"d2e_src1") : Bit RegFileSz <- #src1 ;
+       Write (instancePrefix--"d2e_src2") : Bit RegFileSz <- #src2 ;
+       Write (instancePrefix--"d2e_dst") : Bit RegFileSz <- #dst ;
+       Write (instancePrefix--"pc") : Bit PgmSz <- (#pc_v + $$ (* intwidth *) (natToWord PgmSz 1))  ;
         Retv ) (* rule decode *)
 
     with Rule instancePrefix--"executeArith" :=
     (
-        Read d2eFifo_valid_v : Bool <- d2eFifo_valid ;
-        Read e2wFifo_valid_v : Bool <- e2wFifo_valid ;
-        (* Read sbFlags_v : Array NumRegs Bool <- sbFlags ; *)
+        Read rf_v : Array NumRegs (Bit DataSz) <- (instancePrefix--"rf") ;
 
-        Read d2e_addr_v    : Bit AddrSz    <- d2eFifo_addr ;
-        Read d2e_arithOp_v : OpArithK      <- d2eFifo_arithOp ;
-        Read d2e_op_v      : OpK           <- d2eFifo_op ;
-        Read d2e_pc_v      : Bit PgmSz     <- d2eFifo_pc ;
-        Read d2e_dst_v     : Bit RegFileSz <- d2eFifo_dst ;
-        Read d2e_src1_v    : Bit RegFileSz <- d2eFifo_src1 ;
-        Read d2e_src2_v    : Bit RegFileSz <- d2eFifo_src2 ;
+	Read src1    : Bit RegFileSz <- (instancePrefix--"d2e_src1") ;
+	Read src2    : Bit RegFileSz <- (instancePrefix--"d2e_src2") ;
+	Read dst     : Bit RegFileSz <- (instancePrefix--"d2e_dst") ;
+	Read arithOp : Bit 2 <- (instancePrefix--"d2e_arithOp") ;
+	Read op      : Bit 2 <- (instancePrefix--"d2e_op") ;
+	Read valid   : Bool <- (instancePrefix--"d2e_valid") ;
+        Assert (#op == $$ (* isConstT *)opArith && #valid) ;
 
-        Assert( (#d2e_op_v == $$ (* isConstT *)opArith)
-	      (* && (!(#sbFlags_v @[ #d2e_src1_v ])) *)
-	      (*  && (!(#sbFlags_v @[ #d2e_src2_v ])) *)
-	       && #d2eFifo_valid_v && (!#e2wFifo_valid_v)) ;
-               Write d2eFifo_valid : Bool <- ($$false)%kami_expr ;
-               LET src1 : Bit RegFileSz (* non-call varbinding *) <- #d2e_src1_v ;
-               LET src2 : Bit RegFileSz (* non-call varbinding *) <- #d2e_src2_v ;
-               LET dst : Bit RegFileSz (* non-call varbinding *) <- #d2e_dst_v ;
-               LET arithOp : OpArithK (* non-call varbinding *) <- #d2e_arithOp_v ;
-       Read regsval : Array NumRegs (Bit DataSz) <- rf ;
-       LET val1 : Bit DataSz (* varbinding *) <-  #regsval @[ #src1 ] ;
-       LET val2 : Bit DataSz (* varbinding *) <-  #regsval @[ #src2 ] ;
-
-       LET execVal : Bit DataSz <- (execArith exec _ arithOp val1 val2) ;
-               (* LET flags : Array NumRegs Bool (* non-call varbinding *) <- #sbFlags_v ;
-               LET flags : Array NumRegs Bool <- #flags @[#dst <- $$true ] ;
-               Write sbFlags : Array NumRegs Bool <- #flags ; *)
-               Write e2wFifo_idx : Bit RegFileSz <- #dst ;
-               Write e2wFifo_val : Bit DataSz <- #execVal ;
-               Write e2wFifo_valid : Bool <- ($$true)%kami_expr ;
+	LET val1 : Bit DataSz (* non-call varbinding *) <- (#rf_v @[ #src1 ]) ;
+	LET val2 : Bit DataSz (* non-call varbinding *) <- (#rf_v @[ #src2 ]) ;
+        LET execVal : Bit DataSz <- (execArith exec _ arithOp val1 val2)  ;
+	BKCall enq : Void (* actionBinding *) <- (e2wfifo--"enq") ((#execVal) : Bit DataSz)  ;
         Retv ) (* rule executeArith *)
-
     }). (* mkDecExecSep *)
 
-    Close Scope kami_expr.
-
     Hint Unfold mkDecExecSepModule : ModuleDefs.
-(* Module mkDecExecSep type RegFile#(Bit#(PgmSz), Bit#(InstrSz)) -> Decoder -> Executer -> ProcRegs -> Memory -> ToHost -> Module#(Empty) return type Decoder *)
-    Definition mkDecExecSep := Build_Empty mkDecExecSepModule.
+(* Module mkDecExecSep type RegFile#(Bit#(PgmSz), Bit#(InstrSz)) -> Decoder -> Executer -> Memory -> Reg#(Vector#(NumRegs, Bit#(DataSz))) -> ToHost -> Module#(NoMethods) return type Decoder *)
+    Definition mkDecExecSep := Build_NoMethods mkDecExecSepModule.
     Hint Unfold mkDecExecSep : ModuleDefs.
     Hint Unfold mkDecExecSepModule : ModuleDefs.
 
@@ -219,4 +141,3 @@ Definition mkDecExecSep := module'mkDecExecSep.mkDecExecSep.
 Hint Unfold mkDecExecSep : ModuleDefs.
 Hint Unfold module'mkDecExecSep.mkDecExecSep : ModuleDefs.
 Hint Unfold module'mkDecExecSep.mkDecExecSepModule : ModuleDefs.
-
